BasicC64Semantics defined

bedrock2/src/BasicC64Semantics.v
@@ -1,7 +1,8 @@
 Require Import bedrock2.BasicC64Syntax bedrock2.Semantics.
-Require bedrock2.String.
+Require bedrock2.String bedrock2.Map.UnorderedList.
 Require bbv.Word.
 
+Local Definition shiftWidth s := Word.wordToNat (Word.wand s (Word.NToWord 64 63)).
 Instance parameters : parameters := {|
   syntax := StringNames.Syntax.make BasicC64Syntax.parameters;
   word := Word.word 64;
@@ -9,12 +10,26 @@ Instance parameters : parameters := {|
   word_succ := Word.wplus (Word.wone 64);
   word_test w := if Word.weq (Word.wzero 64) w then false else true;
   word_of_Z w := Some (Word.ZToWord 64 w);
-  interp_binop := _;
+  interp_binop bop :=
+    match bop with
+    | bopname.add => @Word.wplus _
+    | bopname.sub => @Word.wminus _
+    | bopname.and => @Word.wand _
+    | bopname.or => @Word.wor _
+    | bopname.xor => @Word.wxor _
+    | bopname.sru => fun w s => Word.wrshift' w (shiftWidth s)
+    | bopname.slu => fun w s => Word.wlshift' w (shiftWidth s)
+    | bopname.srs => fun w s => Word.wrshifta' w (shiftWidth s)
+    | bopname.ltu => fun a b => if Word.wltb a b then Word.wone 64 else Word.wzero 64
+    | bopname.lts => fun a b => if Word.wsltb a b then Word.wone 64 else Word.wzero 64 
+    | bopname.eq => fun a b => if Word.weq a b then Word.wone 64 else Word.wzero 64
+    end;
+  (* TODO: bedrock2.Byte, bedrock2.Word8 *)
   byte := Word.word 8;
   combine _ b w := Word.wor (Word.wlshift' w 8) (Word.zext b (64-8));
   split _ w := (Word.split1 8 (64-8) w, Word.zext (Word.split2 8 (64-8) w) 8);
-  mem := _;
-  locals := _;
+  (* TODO: faster maps *)
+  mem := UnorderedList.map {| UnorderedList.key_eqb a b := if Word.weq a b then true else false |};
+  locals := UnorderedList.map {| UnorderedList.key_eqb := String.eqb |};
   funname_eqb := String.eqb;
 |}.
-Admitted.
