bedrock2/src/Map/UnorderedList.v
@@ -1,0 +1,22 @@
+Require Import bedrock2.Macros bedrock2.Map.
+Require Coq.Lists.List.
+
+Class parameters := {
+  key : Type;
+  value : Type;
+  key_eqb : key -> key -> bool
+}.
+
+Section UnorderedList.
+  Context {p : unique! parameters}.
+  Instance map : map key value := {|
+    map.rep := list (key * value);
+    map.empty := nil;
+    map.get m k := match List.find (fun p => key_eqb k (fst p)) m with
+                   | Some (_, v) => Some v
+                   | None => None
+                   end;
+    map.put m k v := (cons (k, v) (List.filter (fun p => negb (key_eqb k (fst p))) m))
+  |}.
+End UnorderedList.
+Arguments map : clear implicits.
